Equivalence values , Eisbach method + part1 of TH 11.3.1 except for beta rule which requires extra lemma commute_shift_L

2016/Extended_Typed_Lambda_Calculus.thy
@@ -2,6 +2,8 @@
 theory Extended_Typed_Lambda_Calculus
 imports
   Main
+  "~~/src/HOL/Eisbach/Eisbach"
+  "~~/src/HOL/Eisbach/Eisbach_Tools"
   "$AFP/List-Index/List_Index" 
 begin
 (*>*)
@@ -27,17 +29,18 @@ datatype ltype =
   Unit |
   Fun (domain: ltype) (codomain: ltype) (infixr "\<rightarrow>" 225)
 
-datatype lterm =
+(* internal language definition with Unit only*)
+datatype ltermI =
   LTrue |
   LFalse |
-  LIf (bool_expr: lterm) (then_expr: lterm) (else_expr: lterm) |
+  LIf (bool_expr: ltermI) (then_expr: ltermI) (else_expr: ltermI) |
   LVar nat |
-  LAbs (arg_type: ltype) (body: lterm) |
-  LApp lterm lterm |
+  LAbs (arg_type: ltype) (body: ltermI) |
+  LApp ltermI ltermI |
   unit
 
 
-primrec shift_L :: "int \<Rightarrow> nat \<Rightarrow> lterm \<Rightarrow> lterm" where
+primrec shift_L :: "int \<Rightarrow> nat \<Rightarrow> ltermI \<Rightarrow> ltermI" where
   "shift_L d c LTrue = LTrue" |
   "shift_L d c LFalse = LFalse" |
   "shift_L d c (LIf t1 t2 t3) = LIf (shift_L d c t1) (shift_L d c t2) (shift_L d c t3)" |
@@ -46,7 +49,7 @@ primrec shift_L :: "int \<Rightarrow> nat \<Rightarrow> lterm \<Rightarrow> lter
   "shift_L d c (LApp t1 t2) = LApp (shift_L d c t1) (shift_L d c t2)" |
   "shift_L d c unit = unit"
 
-primrec subst_L :: "nat \<Rightarrow> lterm \<Rightarrow> lterm \<Rightarrow> lterm" where
+primrec subst_L :: "nat \<Rightarrow> ltermI \<Rightarrow> ltermI \<Rightarrow> ltermI" where
   "subst_L j s LTrue = LTrue" |
   "subst_L j s LFalse = LFalse" |
   "subst_L j s (LIf t1 t2 t3) = LIf (subst_L j s t1) (subst_L j s t2) (subst_L j s t3)" |
@@ -56,7 +59,7 @@ primrec subst_L :: "nat \<Rightarrow> lterm \<Rightarrow> lterm \<Rightarrow> lt
   "subst_L j s unit = unit"
 
 (* unit is a value*)
-inductive is_value_L :: "lterm \<Rightarrow> bool" where
+inductive is_value_L :: "ltermI \<Rightarrow> bool" where
   "is_value_L LTrue" |
   "is_value_L LFalse" |
   "is_value_L (LAbs T' t)" |
@@ -67,10 +70,10 @@ inductive is_value_L :: "lterm \<Rightarrow> bool" where
   so we will only consider shifted term t2 (always a valid term)
 *)
 
-abbreviation sequence :: "lterm\<Rightarrow>lterm\<Rightarrow>lterm" (infix ";" 200) where
+abbreviation sequence :: "ltermI\<Rightarrow>ltermI\<Rightarrow>ltermI" (infix ";" 200) where
  "sequence t1 t2 \<equiv> (LApp (LAbs Unit  (shift_L 1 0 t2)) t1)"
 
-primrec FV :: "lterm \<Rightarrow> nat set" where
+primrec FV :: "ltermI \<Rightarrow> nat set" where
   "FV LTrue = {}" |
   "FV LFalse = {}" |
   "FV (LIf t1 t2 t3) = FV t1 \<union> FV t2 \<union> FV t3" |
@@ -80,7 +83,7 @@ primrec FV :: "lterm \<Rightarrow> nat set" where
   "FV unit = {}"
 
 
-inductive eval1_L :: "lterm \<Rightarrow> lterm \<Rightarrow> bool" where
+inductive eval1_L :: "ltermI \<Rightarrow> ltermI \<Rightarrow> bool" where
   -- "Rules relating to the evaluation of Booleans"
   eval1_LIf_LTrue:
     "eval1_L (LIf LTrue t2 t3) t2" |
@@ -108,7 +111,7 @@ abbreviation elem' :: "(nat \<times> ltype) \<Rightarrow> lcontext \<Rightarrow>
   "elem' p \<Gamma> \<equiv> fst p < length \<Gamma> \<and> snd p = nth \<Gamma> (fst p)"
 
 (* had new typing rule for unit and sequence*)
-inductive has_type_L :: "lcontext \<Rightarrow> lterm \<Rightarrow> ltype \<Rightarrow> bool" ("((_)/ \<turnstile> (_)/ |:| (_))" [150, 150, 150] 150) where
+inductive has_type_L :: "lcontext \<Rightarrow> ltermI \<Rightarrow> ltype \<Rightarrow> bool" ("((_)/ \<turnstile> (_)/ |:| (_))" [150, 150, 150] 150) where
   -- "Rules relating to the type of Booleans"
   has_type_LTrue:
     "\<Gamma> \<turnstile> LTrue |:| Bool" |
@@ -123,7 +126,9 @@ inductive has_type_L :: "lcontext \<Rightarrow> lterm \<Rightarrow> ltype \<Righ
   has_type_LAbs:
     "(\<Gamma> |,| T1) \<turnstile> t2 |:| T2 \<Longrightarrow> \<Gamma> \<turnstile> (LAbs T1 t2) |:| (T1 \<rightarrow> T2)" |
   has_type_LApp:
-    "\<Gamma> \<turnstile> t1 |:| (T11 \<rightarrow> T12) \<Longrightarrow> \<Gamma> \<turnstile> t2 |:| T11 \<Longrightarrow> \<Gamma> \<turnstile> (LApp t1 t2) |:| T12" 
+    "\<Gamma> \<turnstile> t1 |:| (T11 \<rightarrow> T12) \<Longrightarrow> \<Gamma> \<turnstile> t2 |:| T11 \<Longrightarrow> \<Gamma> \<turnstile> (LApp t1 t2) |:| T12" |
+  has_type_LUnit:
+    "\<Gamma> \<turnstile> unit |:| Unit"
 
 lemma[simp]: "nat (int x + 1) = Suc x" by simp
 lemma[simp]: "nat (1 + int x) = Suc x" by simp
@@ -135,14 +140,14 @@ lemma gr_Suc_conv: "Suc x \<le> n \<longleftrightarrow> (\<exists>m. n = Suc m \
 
 lemma FV_shift:
   "FV (shift_L (int d) c t) = image (\<lambda>x. if x \<ge> c then x + d else x) (FV t)"
-proof (induction t arbitrary: c rule: lterm.induct)
+proof (induction t arbitrary: c rule: ltermI.induct)
   case (LAbs T t)
   thus ?case by (auto simp: gr_Suc_conv image_iff) force+
 qed auto
 
 lemma FV_subst:
   "FV (subst_L n t u) = (if n \<in> FV u then (FV u - {n}) \<union> FV t else FV u)"
-proof (induction u arbitrary: n t rule: lterm.induct)
+proof (induction u arbitrary: n t rule: ltermI.induct)
   case (LAbs T u)
   thus ?case 
     by (auto simp: gr0_conv_Suc image_iff FV_shift[of 1, unfolded int_1],
@@ -161,7 +166,7 @@ lemma inversion:
   "\<Gamma> \<turnstile> LApp t1 t2 |:| R \<Longrightarrow> \<exists>T11. \<Gamma> \<turnstile> t1 |:| T11 \<rightarrow> R \<and> \<Gamma> \<turnstile> t2 |:| T11"
   "\<Gamma> \<turnstile>  unit |:| R \<Longrightarrow> R = Unit"
   by (auto elim: has_type_L.cases)
-   
+  
 
 theorem uniqueness_of_types:
   "\<Gamma> \<turnstile> t |:| T1 \<Longrightarrow> \<Gamma> \<turnstile> t |:| T2 \<Longrightarrow> T1 = T2"
@@ -183,12 +188,22 @@ proof (induction "insert_nth n U \<Gamma>" t A arbitrary: \<Gamma> n rule: has_t
     by (fastforce intro: has_type_L.intros has_type_LAbs.hyps(2)[where n="Suc n"])+
 qed (fastforce intro: has_type_L.intros simp: nth_append min_def)+
 
+lemma weakening:
+  "\<Gamma> \<turnstile> t |:| A \<Longrightarrow> n \<le> length \<Gamma> \<Longrightarrow> insert_nth n S \<Gamma> \<turnstile> shift_L 1 n t |:| A"
+proof (induction \<Gamma> t A arbitrary: n rule: has_type_L.induct)
+  case (has_type_LAbs \<Gamma> T1 t2 T2)
+  from has_type_LAbs.prems has_type_LAbs.hyps
+    has_type_LAbs.IH[where n="Suc n"] show ?case
+    by (auto intro: has_type_L.intros)
+qed (auto simp: nth_append min_def intro: has_type_L.intros)
+
+
 (* sequence specific lemmas 
     evaluation
     typing
 *)
 
-lemma eval1_Lseq: 
+theorem eval1_Lseq: 
   "eval1_L t1 t1' \<Longrightarrow> eval1_L (t1;t2) (t1';t2)"
   by (auto intro: eval1_L.intros is_value_L.intros)
 
@@ -198,19 +213,16 @@ by (induction t arbitrary:t1 x, force+)
 lemma shift_shift_invert: "a>0 \<Longrightarrow> shift_L (-a) b (shift_L a b t) = t"
 by(induction t arbitrary: a b, auto)
 
-lemma eval1_Lseq_next:
-  "0\<notin>FV t2 \<Longrightarrow> eval1_L (unit ; t2) t2"
-proof -
-  assume H:"0\<notin>FV t2"
-  
+theorem eval1_Lseq_next:
+  " eval1_L (unit ; t2) t2"
+proof -  
   have A:"eval1_L (unit ; t2) (shift_L (-1) 0 (subst_L 0 (shift_L 1 0 unit) (shift_L 1 0 t2)))"
     using eval1_LApp_LAbs
           "is_value_L.simps"
      by presburger
 
   have " subst_L 0 (shift_L 1 0 unit) (shift_L 1 0 t2) = (shift_L 1 0 t2)"
-      using subst_free_var_only[of 0 "shift_L (int 1) 0 t2" "unit"] 
-            H 
+      using subst_free_var_only[of 0 "shift_L (int 1) 0 t2" "unit"]  
             FV_shift[of 1 0 t2]
             image_iff
       by auto
@@ -219,4 +231,187 @@ proof -
     by force        
 qed    
 
+theorem has_type_LSeq: 
+  "\<Gamma> \<turnstile> t1 |:| Unit \<Longrightarrow> \<Gamma> \<turnstile> t2 |:| A \<Longrightarrow> \<Gamma> \<turnstile> (t1 ; t2) |:| A"
+    by (metis insert_nth.simps(1) less_eq_nat.simps(1) has_type_LAbs has_type_LApp
+        weakening)
 
+(* external language definition with sequence as a term*)
+datatype ltermE =
+  LETrue |
+  LEFalse |
+  LEIf (bool_expr: ltermE) (then_expr: ltermE) (else_expr: ltermE) |
+  LEVar nat |
+  LEAbs (arg_type: ltype) (body: ltermE) |
+  LEApp ltermE ltermE |
+  unitE |
+  SeqE (fp: ltermE) (sp: ltermE)
+
+primrec shift_LE :: "int \<Rightarrow> nat \<Rightarrow> ltermE \<Rightarrow> ltermE" where
+  "shift_LE d c LETrue = LETrue" |
+  "shift_LE d c LEFalse = LEFalse" |
+  "shift_LE d c (LEIf t1 t2 t3) = LEIf (shift_LE d c t1) (shift_LE d c t2) (shift_LE d c t3)" |
+  "shift_LE d c (LEVar k) = LEVar (if k < c then k else nat (int k + d))" |
+  "shift_LE d c (LEAbs T' t) = LEAbs T' (shift_LE d (Suc c) t)" |
+  "shift_LE d c (LEApp t1 t2) = LEApp (shift_LE d c t1) (shift_LE d c t2)" |
+  "shift_LE d c unitE = unitE" |
+  "shift_LE d c (SeqE t1 t2) = SeqE (shift_LE d c t1) (shift_LE d (Suc c) t2)"
+
+primrec subst_LE :: "nat \<Rightarrow> ltermE \<Rightarrow> ltermE \<Rightarrow> ltermE" where
+  "subst_LE j s LETrue = LETrue" |
+  "subst_LE j s LEFalse = LEFalse" |
+  "subst_LE j s (LEIf t1 t2 t3) = LEIf (subst_LE j s t1) (subst_LE j s t2) (subst_LE j s t3)" |
+  "subst_LE j s (LEVar k) = (if k = j then s else LEVar k)" |
+  "subst_LE j s (LEAbs T' t) = LEAbs T' (subst_LE (Suc j) (shift_LE 1 0 s) t)" |
+  "subst_LE j s (LEApp t1 t2) = LEApp (subst_LE j s t1) (subst_LE j s t2)" |
+  "subst_LE j s unitE = unitE" |
+  "subst_LE j s (SeqE t1 t2) = SeqE (subst_LE j s t1) (subst_LE j s t2)"
+  
+(* unit is a value*)
+inductive is_value_LE :: "ltermE \<Rightarrow> bool" where
+  "is_value_LE LETrue" |
+  "is_value_LE LEFalse" |
+  "is_value_LE (LEAbs T' t)" |
+  "is_value_LE unitE"
+
+primrec FVE :: "ltermE \<Rightarrow> nat set" where
+  "FVE LETrue = {}" |
+  "FVE LEFalse = {}" |
+  "FVE (LEIf t1 t2 t3) = FVE t1 \<union> FVE t2 \<union> FVE t3" |
+  "FVE (LEVar x) = {x}" |
+  "FVE (LEAbs T1 t) = image (\<lambda>x. x - 1) (FVE t - {0})" |
+  "FVE (LEApp t1 t2) = FVE t1 \<union> FVE t2" |
+  "FVE unitE = {}" |
+  "FVE (SeqE t1 t2) = FVE t1 \<union> FVE t2"
+
+inductive eval1_LE :: "ltermE \<Rightarrow> ltermE \<Rightarrow> bool" where
+  -- "Rules relating to the evaluation of Booleans"
+  eval1_LEIf_LTrue:
+    "eval1_LE (LEIf LETrue t2 t3) t2" |
+  eval1_LEIf_LFalse:
+    "eval1_LE (LEIf LEFalse t2 t3) t3" |
+  eval1_LEIf:
+    "eval1_LE t1 t1' \<Longrightarrow> eval1_LE (LEIf t1 t2 t3) (LEIf t1' t2 t3)" |
+
+  -- "Rules relating to the evaluation of function application"
+  eval1_LEApp1:
+    "eval1_LE t1 t1' \<Longrightarrow> eval1_LE (LEApp t1 t2) (LEApp t1' t2)" |
+  eval1_LEApp2:
+    "is_value_LE v1 \<Longrightarrow> eval1_LE t2 t2' \<Longrightarrow> eval1_LE (LEApp v1 t2) (LEApp v1 t2')" |
+  eval1_LEApp_LEAbs:
+    "is_value_LE v2 \<Longrightarrow> eval1_LE (LEApp (LEAbs T' t12) v2)
+      (shift_LE (-1) 0 (subst_LE 0 (shift_LE 1 0 v2) t12))" |
+  
+  -- "Rules relating to evaluation of sequence"
+  
+  eval1_LE_E_Seq:
+    "eval1_LE t1 t1' \<Longrightarrow> eval1_LE (SeqE t1 t2) (SeqE t1' t2)" |
+  eval1_LE_E_Seq_Next:
+    "eval1_LE (SeqE unitE t2) t2"
+
+(* had new typing rule for unit and sequence*)
+inductive has_type_LE :: "lcontext \<Rightarrow> ltermE \<Rightarrow> ltype \<Rightarrow> bool" ("((_)/ \<turnstile>\<^sup>E (_)/ |:| (_))" [150, 150, 150] 150) where
+  -- "Rules relating to the type of Booleans"
+  has_type_LETrue:
+    "\<Gamma> \<turnstile>\<^sup>E LETrue |:| Bool" |
+  has_type_LEFalse:
+    "\<Gamma> \<turnstile>\<^sup>E LEFalse |:| Bool" |
+  has_type_LEIf:
+    "\<Gamma> \<turnstile>\<^sup>E t1 |:| Bool \<Longrightarrow> \<Gamma> \<turnstile>\<^sup>E t2 |:| T' \<Longrightarrow> \<Gamma> \<turnstile>\<^sup>E t3 |:| T' \<Longrightarrow> \<Gamma> \<turnstile>\<^sup>E (LEIf t1 t2 t3) |:| T'" |
+
+  -- \<open>Rules relating to the type of the constructs of the $\lambda$-calculus\<close>
+  has_type_LEVar:
+    "(x, T') |\<in>| \<Gamma> \<Longrightarrow> \<Gamma> \<turnstile>\<^sup>E (LEVar x) |:| (T')" |
+  has_type_LEAbs:
+    "(\<Gamma> |,| T1) \<turnstile>\<^sup>E t2 |:| T2 \<Longrightarrow> \<Gamma> \<turnstile>\<^sup>E (LEAbs T1 t2) |:| (T1 \<rightarrow> T2)" |
+  has_type_LEApp:
+    "\<Gamma> \<turnstile>\<^sup>E t1 |:| (T11 \<rightarrow> T12) \<Longrightarrow> \<Gamma> \<turnstile>\<^sup>E t2 |:| T11 \<Longrightarrow> \<Gamma> \<turnstile>\<^sup>E (LEApp t1 t2) |:| T12" |
+  
+  has_type_LEUnit:
+    "\<Gamma> \<turnstile>\<^sup>E unitE |:| Unit " |  
+  -- "Rule relating to sequence"
+  has_type_LESeqE:
+    "\<Gamma> \<turnstile>\<^sup>E t1 |:| Unit \<Longrightarrow> \<Gamma> \<turnstile>\<^sup>E t2 |:| A \<Longrightarrow> \<Gamma> \<turnstile>\<^sup>E (SeqE t1 t2) |:| A"
+
+lemma inversionE:
+  "\<Gamma> \<turnstile>\<^sup>E LETrue |:| R \<Longrightarrow> R = Bool"
+  "\<Gamma> \<turnstile>\<^sup>E LEFalse |:| R \<Longrightarrow> R = Bool"
+  "\<Gamma> \<turnstile>\<^sup>E LEIf t1 t2 t3 |:| R \<Longrightarrow> \<Gamma> \<turnstile>\<^sup>E t1 |:| Bool \<and> \<Gamma> \<turnstile>\<^sup>E t2 |:| R \<and> \<Gamma> \<turnstile>\<^sup>E t3 |:| R"
+  "\<Gamma> \<turnstile>\<^sup>E LEVar x |:| R \<Longrightarrow> (x, R) |\<in>| \<Gamma>"
+  "\<Gamma> \<turnstile>\<^sup>E LEAbs T1 t2 |:| R \<Longrightarrow> \<exists>R2. R = T1 \<rightarrow> R2 \<and> \<Gamma> |,| T1 \<turnstile>\<^sup>E t2 |:| R2"
+  "\<Gamma> \<turnstile>\<^sup>E LEApp t1 t2 |:| R \<Longrightarrow> \<exists>T11. \<Gamma> \<turnstile>\<^sup>E t1 |:| T11 \<rightarrow> R \<and> \<Gamma> \<turnstile>\<^sup>E t2 |:| T11"
+  "\<Gamma> \<turnstile>\<^sup>E unitE |:| R \<Longrightarrow> R = Unit"
+  "\<Gamma> \<turnstile>\<^sup>E SeqE t1 t2 |:| R \<Longrightarrow> \<exists>A. R = A \<and> \<Gamma> \<turnstile>\<^sup>E t2 |:| A \<and> \<Gamma> \<turnstile>\<^sup>E t1 |:| Unit"
+  by (auto elim: has_type_LE.cases)
+
+
+lemma canonical_formsE:
+  "is_value_LE v \<Longrightarrow> \<Gamma> \<turnstile>\<^sup>E v |:| Bool \<Longrightarrow> v = LETrue \<or> v = LEFalse"
+  "is_value_LE v \<Longrightarrow> \<Gamma> \<turnstile>\<^sup>E v |:| T1 \<rightarrow> T2 \<Longrightarrow> \<exists>t. v = LEAbs T1 t"
+  "is_value_LE v \<Longrightarrow> \<Gamma> \<turnstile>\<^sup>E v |:| Unit \<Longrightarrow> v = unitE"
+by (auto elim: has_type_LE.cases is_value_LE.cases)
+  
+
+lemma weakeningE:
+  "\<Gamma> \<turnstile>\<^sup>E t |:| A \<Longrightarrow> n \<le> length \<Gamma> \<Longrightarrow> insert_nth n S \<Gamma> \<turnstile>\<^sup>E shift_LE 1 n t |:| A"
+proof (induction \<Gamma> t A arbitrary: n rule: has_type_LE.induct)
+  case (has_type_LEAbs \<Gamma> T1 t2 T2)
+  from has_type_LEAbs.prems has_type_LEAbs.hyps
+    has_type_LEAbs.IH[where n="Suc n"] show ?case
+    by (auto intro: has_type_LE.intros)
+qed (auto simp: nth_append min_def intro: has_type_LE.intros)
+ 
+(* Theorem 11.3.1 Sequence is a derived form*)
+
+(*e is a translation function from external to internal language*)
+
+
+fun e::"ltermE \<Rightarrow> ltermI" where
+  "e LETrue = LTrue" |
+  "e LEFalse = LFalse" |
+  "e (LEIf t1 t2 t3) = LIf (e t1) (e t2) (e t3)" |
+  "e (LEVar x) = LVar x" |
+  "e (LEAbs A t1) = LAbs A (e t1)" |
+  "e (LEApp t1 t2) = LApp (e t1) (e t2)" |
+  "e unitE = unit" |
+  "e (SeqE t1 t2) = (e t1 ; e t2)"
+
+(* 
+  This theorem shows that both implementation of sequence are
+   equivalent in term of typing and evaluation
+*)
+
+lemma e_comp_shift: "e (shift_LE d c t) = shift_L d c (e t)"
+proof (induction arbitrary: d c rule: e.induct)
+  case (8 t2 t1)
+    thus ?case
+      apply simp
+qed auto
+  
+method e_elim uses rule1 = (auto intro: e.elims[OF rule1] is_value_LE.intros) 
+method sym_then_elim = match premises in I: "A = B" for A and B \<Rightarrow>
+            \<open>e_elim rule1: HOL.sym[OF I]\<close>
+
+lemma value_equiv: "is_value_LE v1 \<longleftrightarrow> is_value_L (e v1)" (is "?P \<longleftrightarrow> ?Q")
+proof
+  show "?P \<Longrightarrow> ?Q"
+    by (induction rule: is_value_LE.induct, auto intro:"is_value_L.intros")    
+next
+  show "?Q \<Longrightarrow> ?P" 
+    by (induction "e v1" rule: is_value_L.induct, sym_then_elim+)
+qed
+
+theorem equiv_eval :
+ "eval1_LE t t' \<longleftrightarrow> eval1_L (e t) (e t')" (is "?P \<longleftrightarrow> ?Q")
+proof 
+  show "?P \<Longrightarrow> ?Q"
+    proof (induction rule:eval1_LE.induct)
+      case (eval1_LEApp2 v1 t2 t2')
+        thus ?case by (metis e.simps(6) value_equiv eval1_L.intros(5))
+    next
+      case (eval1_LEApp_LEAbs v1 A t)
+        thus ?case
+          sorry
+          
+    qed (auto intro: eval1_L.intros eval1_Lseq eval1_Lseq_next)
+next
